theories/arjen.v
@@ -1,0 +1,159 @@
+Require Coq.Lists.List.
+From iris.proofmode Require Import tactics.
+Open Scope type_scope.
+
+Definition Associative {T : Type} (R : T -> T -> T -> Type) : Type :=
+  forall a b ab c abc, R a b ab -> R ab c abc -> sigT (fun bc => (R a bc abc) * (R b c bc)).
+
+Section ListSplit.
+  Context {T : Type}.
+  Context (Tsplit : T -> T -> T -> Type).
+
+  Inductive listsplit : list T -> list T -> list T -> Type :=
+  | divide : forall x x1 x2 xs ys zs , listsplit xs ys zs -> Tsplit x1 x2 x -> listsplit (x1 :: xs) (x2 :: ys) (x :: zs)
+  | consl   : forall x xs ys zs , listsplit xs ys zs -> listsplit (x :: xs) ys (x :: zs)
+  | consr  : forall x xs ys zs , listsplit xs ys zs -> listsplit xs (x :: ys) (x :: zs)
+  | nill : listsplit nil nil nil.
+
+
+  Hint Resolve divide consl consr nill : listsplit.
+  Ltac inv H := inversion H; clear H; subst.
+
+  Lemma listsplit_assoc : Associative Tsplit -> Associative listsplit.
+  Proof.
+    intros A ????? L1 L2.
+    revert a b L1.
+    induction L2; intros;[
+        inv L1; destruct (IHL2 _ _ X) as [? []]; eauto with listsplit;
+        destruct (A _ _ _ _ _ X0 t) as [? []]
+      | inv L1; destruct (IHL2 _ _ X) as [? []]
+      | destruct (IHL2 _ _ L1) as [? []]
+      | inv L1
+    ]; eauto with listsplit.
+  Qed.
+End ListSplit.
+
+Section ListSplit.
+  Context (S : Type).
+
+  Inductive semptiness : S -> S -> S -> Type :=.
+  Inductive scopy : S -> S -> S -> Type :=
+    | copy : forall x, scopy x x x.
+
+  Definition disjoint : list S -> list S -> list S -> Type :=
+    listsplit semptiness.
+
+  Definition overlaps : list S -> list S -> list S -> Type :=
+    listsplit scopy.
+
+  Inductive permute : list S -> list S -> Type :=
+    | refl : forall xs, permute xs xs
+    | prep : forall x xs ys, permute xs ys -> permute (x :: xs) (x :: ys)
+    | swap : forall x y xs ys, permute xs ys -> permute (x :: y :: xs) (y :: x :: ys)
+    | trans : forall xs ys zs, permute xs ys -> permute ys zs -> permute xs zs.
+
+  Definition module := list S * list S.
+
+  Definition exchange : list S -> list S -> module -> Type := fun d u m =>
+      sigT (fun e => sigT (fun e' =>
+      (disjoint (snd m) e d) *
+      (overlaps (fst m) e' u) *
+      permute e e')).
+
+  Inductive modulesplit : module -> module -> module -> Type :=
+    | msplit : forall {u1 d1 u2 d2 u1' d1' u2' d2' u d},
+        exchange d1 u2 (u2' , d2') ->
+        exchange d2 u1 (u1' , d1') ->
+        disjoint u1' u2' u ->
+        overlaps d1' d2' d ->
+        modulesplit (u1 , d1) (u2 , d2) (u , d).
+
+  Ltac inv H := inversion H; clear H; subst.
+  Hint Resolve divide consl consr nill copy refl prep swap trans : listsplit.
+  Ltac simpl_rel := repeat match goal with
+    | H : semptiness _ _ _ |- _ => inv H
+    | H : scopy _ _ _ |- _ => inv H
+    end.
+
+  Lemma xsplit a b c d zs :
+    overlaps a b zs -> disjoint c d zs ->
+    {ac & {ad & {bc & {bd &
+      overlaps ac bc c * overlaps ad bd d *
+      disjoint ac ad a * disjoint bc bd b }}}}.
+  Proof.
+    revert a b c d. induction zs as [|z zs]; intros ???? O D.
+    { inv O. inv D. do 4 eexists; repeat split; constructor. }
+    inv O; inv D; simpl_rel;
+    match goal with
+    | H : listsplit scopy _ _ _, H' : listsplit semptiness _ _ _ |- _ =>
+      destruct (IHzs _ _ _ _ H H') as [? [? [? [? [[[] ?] ?]]]]]
+    end; simpl_rel; do 4 eexists; repeat split;
+    try eassumption; constructor; eauto with listsplit.
+  Qed.
+
+  Lemma same {T} {x} {r : T -> T -> T -> Type} : listsplit r [] x x.
+  Proof. induction x; eauto with listsplit. Qed.
+
+  Lemma same' {T} {x} {r : T -> T -> T -> Type} : listsplit r x [] x.
+  Proof. induction x; eauto with listsplit. Qed.
+
+  Lemma is_same {T} {x y} {r : T -> T -> T -> Type} : listsplit r [] x y -> x = y.
+  Proof.
+    revert y.
+    induction x.
+    - intros. inv X. reflexivity.
+    - intros. inv X. specialize (IHx _ X0). subst. reflexivity.
+  Qed.
+
+  Lemma is_same' {T} {x y} {r : T -> T -> T -> Type} : listsplit r x [] y -> x = y.
+  Proof.
+    revert y.
+    induction x.
+    - intros. inv X. reflexivity.
+    - intros. inv X. specialize (IHx _ X0). subst. reflexivity.
+  Qed.
+
+  Fixpoint xup a b ab c bc :
+    disjoint a b ab → overlaps b c bc →
+    sigT (fun abc => disjoint a bc abc * overlaps ab c abc).
+  Proof.
+    intros D O.
+    inversion D; inversion O; subst; simpl_rel; fold overlaps disjoint in *.
+    - destruct (xup _ _ _ _ _ X O) as [? []].
+      eexists. split; constructor; eassumption.
+    - destruct (xup _ _ _ _ _ X O) as [? []].
+      eexists. split; constructor; eassumption.
+    - destruct (xup _ _ _ _ _ D X0) as [? []].
+      eexists. split; constructor; eassumption.
+    - rewrite (is_same' X). eexists. split; apply same'.
+    - injection H2 as -> ->.
+      destruct (xup _ _ _ _ _ X X0) as [? []].
+      eexists. split; constructor; eassumption || constructor.
+    - injection H2 as -> ->.
+      destruct (xup _ _ _ _ _ X X0) as [? []].
+      eexists. split; constructor; eassumption || constructor.
+    - destruct (xup _ _ _ _ _ D X0) as [? []].
+      eexists. split; constructor; eassumption || constructor.
+    - inv H2.
+    - inv H2.
+    - inv H2. 
+    - pose proof (is_same O). inv H.
+      eexists. split; constructor; try eassumption. apply same.
+    - exists []. split; constructor.
+  Qed.
+
+  Lemma modulesplit_assoc : Associative modulesplit.
+  Proof.
+    unfold Associative.
+    intros.
+    inv X.
+    inv X0.
+    destruct X1,X2,X,X5.
+    destruct s,s0,s1,s2. simpl in *.
+    repeat match goal with
+    H : _ * _ |- _ => destruct H
+    end.
+    eexists.
+    split; econstructor; unfold exchange in *; simpl in *;
+    repeat eexists; repeat split.
+  Qed.
